

Proof that the RSA decryption algorithm works

From the key generation algorithm:

- p and q are prime numbers
- $n = p \cdot q$
- $\phi(n)$ is the totient of n , which can be computed as $n = (p-1) \cdot (q-1)$
 - this computation of $\phi(n)$ comes from the factorization of n into a product of prime numbers
 - http://en.wikipedia.org/wiki/Euler%27s_totient_function
- $d \cdot e \equiv 1 \pmod{\phi(n)}$

Theorem: for all M in $[0; n[$, $(M^e)^d \equiv M \pmod{n}$

Proof:

- Case 1: $\gcd(M, n) = 1$.
 - Euler's Theorem states that if a and n are coprime positive integers, then $a^{\phi(n)} \equiv 1 \pmod{n}$
 - http://en.wikipedia.org/wiki/Euler%27s_theorem
 - since M and n are coprime positive integers, then $M^{\phi(n)} \equiv 1 \pmod{n}$
 - $(M^e)^d \equiv M^{ed} \equiv M^{(1+k\phi(n))} \equiv M \cdot (M^{\phi(n)})^k \equiv M \cdot 1 \equiv M \pmod{n}$
- Case 2: $\gcd(M, n) \neq 1$.
 - The Chinese Remainder Theorem states that if $\gcd(p, q) = 1$, then $x \equiv y \pmod{p}$ and $x \equiv y \pmod{q}$ implies that $x \equiv y \pmod{pq}$
 - Since $\gcd(p, q) = 1$, we will simply show that (1) $M^{ed} \equiv M \pmod{p}$ and (2) $M^{ed} \equiv M \pmod{q}$ (which will imply that $M^{ed} \equiv M \pmod{pq} = M \pmod{n}$)
 - Since $\gcd(M, n) \neq 1$ and $n = p \cdot q$, we have either $\gcd(M, n) = p$ or $\gcd(M, n) = q$. We assume without loss of generality that $\gcd(M, n) = p$.
 - Since p is a divisor of M , $M = k \cdot p \equiv 0 \pmod{p}$, and $(M^e)^d \equiv M^{ed} \equiv (k^e)^d \cdot (p^e)^d \equiv 0 \pmod{p}$ (the last equality comes from $p^{\dots} \equiv 0 \pmod{p}$)
 - Thus, $M^{ed} \equiv M \pmod{p}$, and the first part is proven
 - $\gcd(M, q) = 1$, thus we can apply Euler's theorem to show that $M^{\phi(q)} \equiv 1 \pmod{q}$, with $\phi(q) = q-1$ as q is prime
 - $(M^e)^d \equiv M^{ed} \equiv M^{(1+k\phi(n))} \equiv M \cdot M^{(k(p-1)(q-1))} \equiv M \cdot (M^{(q-1)})^{(k(p-1))} \equiv M \cdot 1^{(k(p-1))} \equiv M \pmod{q}$, and the second part is proven (the second-to-last equality comes from $M^{(q-1)} \equiv M^{\phi(q)} \equiv 1 \pmod{q}$ thanks to Euler's Theorem)
 - Both parts are proven, which completes the proof of the second case.